Progress

examples/Sec.v
@@ -3,7 +3,7 @@ From Coq Require Import Arith.PeanoNat.
 From CTree Require Import
   CTree.Equ
   CTree.Core
-  Events.Writer
+  CTree.Events.Writer
   Logic.Ctl
   CTree.SBisim
   CTree.Logic.Trans
@@ -27,18 +27,39 @@ Local Open Scope ctl_scope.
 Variant Sec: Set := H | L.
 
 (*| Preorder of [sec] labels |*)
-Reserved Notation "a ≤ b" (at level 52, left associativity).
-Variant sec_preord: rel Sec Sec :=
-| SecRefl: forall a, a ≤ a
-| SecHL: L ≤ H
-where "a ≤ b" := (sec_preord a b).
-Local Hint Constructors sec_preord: core.
+Reserved Notation "a ≺ b" (at level 52, left associativity).
+Variant sec_lt: relation Sec :=
+  | SecLt: L ≺ H
+where "a ≺ b" := (sec_lt a b).
+Local Hint Constructors sec_lt: core.
 
-Local Instance sec_preord_refl: Reflexive sec_preord := SecRefl.
-Local Instance sec_preord_trans: Transitive sec_preord.
+Reserved Notation "a ⪯ b" (at level 52, left associativity).
+Variant sec_lte: relation Sec :=
+| SecRefl: forall a, a ⪯ a
+| SecHL: L ≺ H -> L ⪯ H
+where "a ⪯ b" := (sec_lte a b).
+Local Hint Constructors sec_lte: core.
+
+Local Instance sec_lte_refl: Reflexive sec_lte := SecRefl.
+Local Instance sec_lt_trans: Transitive sec_lt.
+Proof.
+  red; intros [] [] [] *; auto; intros.
+  inv H0. inv H1.
+Qed.
+
+Local Instance sec_lte_trans: Transitive sec_lte.
 Proof. red; intros [] [] [] *; auto. Qed.
 
-Lemma sec_preord_dec(l r: Sec): { l ≤ r } + { r ≤ l }.
+Lemma sec_lt_dec(l r: Sec): { l ≺ r } + { r ⪯ l }.
+Proof.
+  revert r; induction l; destruct r.
+  - right; auto. 
+  - right; auto. 
+  - left; auto.
+  - right; auto. 
+Qed.
+
+Lemma sec_lte_dec(l r: Sec): { l ⪯ r } + { r ⪯ l }.
 Proof.
   revert r; induction l; destruct r.
   - left; reflexivity. 
@@ -64,33 +85,53 @@ Section SecurityEx.
           | Write l addr v => unit
           end.
 
-  Global Instance handler_secE: secE ~> stateT St (ctree void) := {
-      handler e :=
-        mkStateT
-          (fun (st: St) =>                                     
-             match e return ctree void (encode e * St) with
-             | Read l_r addr =>                                 
-                 match lookup addr st with
-                 | Some (l_a, v) =>
-                     if sec_preord_dec l_r l_a then
-                       Ctree.stuck
-                     else
-                       Ret (v, st)
-                 | None => Ret (0%nat, st)
-                 end
-             | Write l_w addr v =>
-                 match lookup addr st with
-                 | Some (l_a, _) =>
-                     if sec_preord_dec l_w l_a then
-                       Ctree.stuck
-                     else
+  Definition h_secE: secE ~> stateT St (ctree void) :=
+    fun e => mkStateT
+            (fun (st: St) =>                                     
+               match e return ctree void (encode e * St) with
+               | Read l_r addr =>                                 
+                   match lookup addr st with
+                   | Some (l_a, v) =>
+                       if sec_lte_dec l_a l_r then
+                         Ret (v, st)
+                       else
+                         Ctree.stuck
+                   | None => Ret (0%nat, st)
+                   end
+               | Write l_w addr v =>
+                   match lookup addr st with
+                   | Some (l_a, _) =>
+                       if sec_lt_dec l_w l_a then
+                         Ctree.stuck
+                       else
+                         Ret (tt, add addr (l_w, v) st)
+                   | None =>
                        Ret (tt, add addr (l_w, v) st)
-                 | None =>
-                     Ret (tt, add addr (l_w, v) st)
-                 end
-             end)
-    }.
+                   end
+               end).
 
+  Record readG :=
+    {
+      m : Addr;
+      ml: Sec;
+      al: Sec;
+    }.
+               
+  (* Instrumented semantics, simply log every read with [readG] *)
+  Definition h_secE_instr: secE ~> stateT St (ctreeW readG) :=
+    h_writerA
+      h_secE
+      (fun (e: secE) (v: encode e) (σ: St) =>
+         match e return option readG with
+         | Read al addr =>
+             match lookup addr σ with
+             | Some (ml, _) => Some {| m:= addr; ml := ml; al := al |}
+             | None => None
+             end
+         | Write _ _ _ => None
+         end).
+
+  (* Trigger instructions *)
   Definition read: Sec -> Addr -> ctree secE nat :=
     fun (l: Sec) (addr: Addr) => @Ctree.trigger secE secE _ _ (ReSum_refl) (ReSumRet_refl) (Read l addr).
   
@@ -98,48 +139,36 @@ Section SecurityEx.
     fun (l: Sec) (addr: Addr) (s: nat) => Ctree.trigger (Write l addr s).
 
   (* Alice (H) writes [secret] to odd addresses *)
-  Definition sec_alice1(secret: nat): ctree secE unit :=
-    i <- read L 0 ;; 
+  Definition sec_alice1(secret: nat)(i: Addr): ctree secE unit :=
     if Nat.Even_Odd_dec i then
       write H (i+1) secret
     else
-      write H i secret ;;
-    write L 0 (S i).
+      write H i secret.
  
   (* Bob (L) reads from even addresses *)
-  Definition sec_bob1: ctree secE unit :=
-    i <- read L 0 ;; 
-    (if Nat.Even_Odd_dec i then
-      read L i 
+  Definition sec_bob1(i: Addr): ctree secE unit :=
+    if Nat.Even_Odd_dec i then
+      read L i;; Ret tt
     else
-      read L (i+1)) ;;
-    write L 0 (S i).
+      read L (i+1) ;; Ret tt.
 
-  Definition sec_system(secret: nat) :=
-    (* start [i:=1] to avoid conflict with counter at address [0] *)
-    write L 0 1 ;;
-    forever (fun _ => brS2 (sec_alice1 secret) sec_bob1) tt.
+  Definition sec_system(secret: nat): ctree secE void :=
+    Ctree.forever void
+      (fun (i: nat) =>
+         (br2
+            (sec_alice1 secret i)
+            (sec_bob1 i));;
+         (* Increase counter by 1 *)
+         Ret (S i)) 0.
 
-  (* Interpret system with handler (handler_stateT_trace handler_secE) *)
-  Definition t_w (secret: nat): ctreeEW secE (unit * St) :=
-    interp_state (h_stateT_writerE handler_secE) (sec_system secret) empty.
-
-  Definition reads_secret(e: Bar secE)(secret: nat) :=
-    match e with
-    | Obs e x =>
-        match e return encode e -> Prop with
-        | Read L addr => fun x: nat => x = secret
-        | _ => fun _ => False
-        end x
-    end.
-  
-  Theorem ctl_safety_sec1: forall (secret: nat) (addr: Addr),
-      secret <> 0 ->
-      <( {(t_w secret, None)}
-           |== AG ¬ now {fun '(Obs (Log e) _) => reads_secret e secret })>.
+  (* Safety property: there does not exist a memory label ml ≺ al, or there does
+     not exist a low intruction that reads from high-security memory *)
+  Theorem ag_safety_sec: forall (secret: nat) (σ: St),
+      <( {interp_state h_secE_instr (sec_system secret) σ}, Pure |= AG visW \s, s.(al) ≺ s.(al) )>.
   Proof.
     intros.
-    Unset Printing Notations.
+    unfold sec_system, forever.
+    
     
     unfold t_w, sec_system.
   Admitted.
