theories/CTree/Logic/EF.v
@@ -1,0 +1,549 @@
+From Coq Require Import
+  Basics
+  Arith.Wf_nat
+  Classes.Morphisms.
+
+From Coinduction Require Import
+  coinduction lattice.
+
+From CTree Require Import
+  Events.Core
+  Events.WriterE
+  CTree.Core
+  CTree.Equ
+  CTree.SBisim
+  CTree.Interp.Core
+  CTree.Interp.State
+  CTree.Logic.Trans
+  CTree.Logic.CanStep
+  Logic.Ctl
+  Logic.AX
+  Logic.Kripke
+  Logic.Setoid.
+
+Set Implicit Arguments.
+Generalizable All Variables.
+
+Import CTreeNotations CtlNotations.
+Local Open Scope ctl_scope.
+Local Open Scope ctree_scope.
+  
+(*| CTL logic lemmas on c/itrees |*)
+Section BasicLemmas.
+  Context {E: Type} {HE: Encode E} {X: Type}.
+
+  Lemma ef_done: forall (t: ctree E X) φ w,
+      is_done w ->
+      <( t, w |= EF now φ )> ->
+      φ w.
+  Proof.
+    intros * Hret Hcontra.
+    inv Hcontra.
+    - now rewrite ctl_now in H.
+    - destruct H0 as (? & ? & ? & ?).
+      exfalso.
+      eapply done_not_ktrans with (t:=t); eauto.
+  Qed.
+
+  Lemma ef_stuck: forall w φ,
+      <( {Ctree.stuck: ctree E X}, w |= EF φ )> <->
+      <( {Ctree.stuck: ctree E X}, w |= φ )>.
+  Proof.
+    split; intros.
+    - cbn in H; rewrite unfold_stuck; dependent induction H; auto.
+      + now rewrite unfold_stuck in H.
+      + destruct H0 as (? & ? & ? & ?).
+        now apply ktrans_stuck in H0.
+    - now next; left.
+  Qed.
+
+  Lemma ef_ret: forall r w (Rr: rel X (World E)),      
+      Rr r w ->
+      not_done w ->
+      <( {Ret r}, w |= EF done Rr )>.
+  Proof.
+    intros * Hr Hd.
+    next; right.
+    next; inv Hd.
+    - exists (Ctree.stuck), (Done r); split.
+      + apply ktrans_done; auto.
+      + apply ef_stuck. now constructor.
+    - exists (Ctree.stuck), (Finish e v r); split.
+      + apply ktrans_finish; auto.
+      + apply ef_stuck; now constructor.
+  Qed.
+
+  Lemma not_done_vis_ef: forall (t: ctree E X) φ w,
+      <( t, w |= EF vis φ )> ->
+      not_done w.
+  Proof with eauto with ctl.
+    intros * Hf.
+    next in Hf ; destruct Hf.
+    - rewrite ctl_vis in H; inv H...
+    - destruct H as (? & ? & ? & ?).
+      now apply ktrans_not_done with t x x0.
+  Qed.
+
+  Lemma not_done_pure_ef: forall (t: ctree E X) w,
+      <( t, w |= EF pure )> ->
+      not_done w.
+  Proof with eauto with ctl.
+    intros * Hf.
+    next in Hf ; destruct Hf.
+    - rewrite ctl_pure in H; subst...
+    - destruct H as (? & ? & ? & ?).
+      now apply ktrans_not_done with t x x0.
+  Qed.
+
+  Lemma ef_guard: forall (t: ctree E X) w φ,
+      <( {Guard t}, w |= EF φ )> <->
+      <( t, w |= EF φ )>.
+  Proof.
+    intros.
+    now rewrite sb_guard.
+  Qed.
+
+  Lemma ef_br: forall n (k: fin' n -> ctree E X) w φ,
+      <( {Br n k}, w |= EF now φ )> <->
+        (exists (i: fin' n), <( {k i}, w |= EF now φ )>).
+  Proof.
+    split; intros.
+    - next in H; destruct H.
+      + exists Fin.F1.
+        next; left.
+        now rewrite ctl_now in *.
+      + destruct H as (? & ? & ? & ?).
+        apply ktrans_br in H as (i & ? & -> & ?).
+        rewrite H in H0.
+        now (exists i).
+    - destruct H as (i & ?).
+      next in H; destruct H.
+      + next; left.
+        now rewrite ctl_now in *.
+      + next; right; next.
+        destruct H as (? & ? & ? & ?).
+        exists (k i), w; split; auto with ctl.
+        * apply ktrans_br.
+          exists i; intuition.
+        * next; right; next.
+          exists x, x0; intuition.
+  Qed.
+
+  Lemma ef_vis: forall (e: E) (k: encode e -> ctree E X) (_: encode e) w φ,
+      (φ w \/ (not_done w /\ exists (x: encode e),
+                 <( {k x}, {Obs e x} |= EF now φ )>)) ->
+      <( {Vis e k}, w |= EF now φ )>.        
+  Proof.
+    intros.
+    destruct H as [H | [Hd (v & ?)]].
+    - now next; left.
+    - next; right; next.
+      + exists (k v), (Obs e v); split; auto.
+        apply ktrans_vis.
+        exists v; intuition.
+  Qed.
+
+  Lemma ef_ret_inv: forall (x: X) w R,
+      <( {Ret x}, w |= EF (EX done R) )> ->
+      R x w.
+  Proof.
+    intros.
+    next in H; destruct H.
+    - destruct H as (? & ? & ? & ?).
+      ddestruction H; now ddestruction H0.
+    - next in H; destruct H as (? & ? & ? & ?).
+      ddestruction H; observe_equ x; next in H0; destruct H0;
+        rewrite <- Eqt, H in H0;
+        destruct H0 as (? & ? & ? & ?);
+        now apply ktrans_stuck in H0.
+  Qed.
+
+End BasicLemmas.
+
+(* TODO: WIP here copied from AF.v *)
+Section CtlEfBind.
+  Context {E: Type} {HE: Encode E}.
+
+  Typeclasses Transparent equ.
+  Theorem af_bind_vis{X Y}: forall (t: ctree E Y) (k: Y -> ctree E X) φ w,
+      <( t, w |= AF vis φ )> ->
+      <( {x <- t ;; k x}, w |= AF vis φ )>.
+  Proof.
+    intros * Haf.
+    revert X k.
+    induction Haf; intros; subst.
+    - (* MatchA *)
+      next; left; cbn.
+      apply ctl_vis in H; inv H; now constructor.
+    - (* StepA *)
+      destruct H0, H1; clear H H0.      
+      next; right; next; split.
+      + (* can_step *)
+        destruct H1 as (t' & w' & TR').
+        eapply can_step_bind_l with t' w'; auto.
+        eapply not_done_vis_af with (t:=t').
+        now apply H2.
+      + (* AX AF *)
+        intros t_ w_ TR_.
+        apply ktrans_bind_inv in TR_ as
+            [(t' & TR' & Hd & ->) |
+              (x & w' & TR' & Hr & TRk)].
+        * now apply H3.
+        * specialize (H2 _ _ TR').
+          inv H2.
+          apply ctl_vis in H; inv H. 
+          -- inv Hr.
+          -- destruct H0.
+             now apply can_step_stuck in H0.
+  Qed.
+
+  Theorem af_bind_pure{X Y}: forall (t: ctree E Y) (k: Y -> ctree E X) w,
+      <( t, w |= AF pure )> ->
+      <( {x <- t ;; k x}, w |= AF pure )>.
+  Proof.
+    intros * Haf.
+    revert X k.
+    induction Haf; intros; subst.
+    - (* MatchA *)
+      next; left; cbn.
+      now apply ctl_pure in H. 
+    - (* StepA *)
+      destruct H0, H1; clear H H0.      
+      next; right; next; split.
+      + (* can_step *)
+        destruct H1 as (t' & w' & TR').
+        eapply can_step_bind_l with t' w'; auto.
+        eapply not_done_pure_af with (t:=t').
+        now apply H2.
+      + (* AX AF *)
+        intros t_ w_ TR_.
+        apply ktrans_bind_inv in TR_.
+        destruct TR_ as [(t' & TR' & Hd & ->) | (x & w' & TR' & Hr & TRk)].
+        * now apply H3.
+        * specialize (H2 _ _ TR').
+          inv H2.
+          apply ctl_pure in H; subst.
+          -- inv Hr.
+          -- destruct H0.
+             now apply can_step_stuck in H0.
+  Qed.
+
+  Theorem af_bind_r{X Y}: forall (t: ctree E Y) (k: Y -> ctree E X) w φ R,
+      <( t, w |= AF AX done R )> ->
+      (forall (y: Y) w, R y w -> not_done w ->
+                   <( {k y}, w |= AF now φ )>) ->
+      <( {x <- t ;; k x}, w |= AF now φ )>.
+  Proof.
+    intros.
+    apply afdone_ind in H.
+    revert H0.
+    generalize dependent φ.
+    generalize dependent k.
+    induction H; intros; observe_equ H; rewrite Eqt.
+    - (* Done *)
+      rewrite bind_ret_l; eauto with ctl.
+    - (* Finish *)
+      rewrite bind_ret_l; eauto with ctl.
+    - (* Tau *)
+      rewrite bind_guard.
+      apply af_guard; eauto with ctl.
+    - (* Vis *)
+      rewrite bind_vis.
+      apply af_vis; eauto with ctl.
+    - (* Br *)
+      rewrite bind_br.
+      apply af_br; eauto with ctl.
+  Qed.
+
+  Lemma af_bind_r_eq{X Y}: forall (t: ctree E Y) (k: Y -> ctree E X) w φ r w',
+      <( t, w |= AF AX done= r w' )> ->
+      <( {k r}, w' |= AF now φ )> ->
+      <( {x <- t ;; k x}, w |= AF now φ )>.
+  Proof.
+    intros.
+    eapply af_bind_r.
+    + apply H.
+    + intros.
+      now destruct H1 as (-> & ->). 
+  Qed.
+  
+End CtlAfBind.
+
+Section CtlAfIter.
+  Context {E: Type} {HE: Encode E}.
+
+  (* Total correctness lemma for [iter] *)
+  (* [Ri: I -> World E -> Prop] loop invariant (left).
+     [Rr: X -> World E -> Prop] loop postcondition (right).
+     [Rv: (I * World E) -> (I * World E) -> Prop)] loop variant (left). *)
+  Lemma af_iter{X I} Ri Rr (Rv: relation (I * World E)) (i: I) w (k: I -> ctree E (I + X)):
+    (forall (i: I) w,
+        Ri i w ->
+        <( {k i}, w |= AF AX done
+                    {fun (x: I + X) w' =>
+                       match x with
+                       | inl i' => Ri i' w' /\
+                                    Rv (i', w') (i, w)
+                       | inr r' => Rr r' w'
+                       end})>) ->
+    well_founded Rv ->
+    Ri i w ->
+    <( {iter k i}, w |= AF done Rr )>.
+  Proof.      
+    intros H WfR Hi.
+    generalize dependent k.
+    revert Hi.
+    remember (i, w) as P.
+    replace i with (fst P) by now subst.
+    replace w with (snd P) by now subst.
+    clear HeqP i w.
+    Opaque entailsF.
+    induction P using (well_founded_induction WfR);
+      destruct P as (i, w); cbn in *. 
+    rename H into HindWf.
+    intros.
+    unfold iter, MonadIter_ctree.
+    rewrite unfold_iter.
+    eapply af_bind_r with
+      (R:=fun (x : I + X) (w' : World E) =>
+            match x with
+            | inl i' => Ri i' w' /\ Rv (i', w') (i, w)
+            | inr r' => Rr r' w'
+            end); auto.
+    intros [i' | r] w'.
+    - intros (Hi' & Hv) Hd.
+      apply af_guard.
+      remember (i', w') as y.
+      replace i' with (fst y) by now subst.
+      replace w' with (snd y) by now subst.      
+      apply HindWf; inv Heqy; auto.
+    - apply af_ret. 
+  Qed.
+
+  (*| Instead of a WF relation [Rv] provide a "ranking" function [f] |*)
+  Lemma af_iter_nat{X I} Ri Rr (f: I -> World E -> nat) (i: I) w (k: I -> ctree E (I + X)):
+    (forall (i: I) w,
+        Ri i w ->
+        <( {k i}, w |= AF AX done
+                    {fun (x: I + X) w' =>
+                       match x with
+                       | inl i' => Ri i' w' /\ f i' w' < f i w
+                       | inr r' => Rr r' w'
+                       end})>) ->
+    Ri i w ->
+    <( {iter k i}, w |= AF done Rr )>.
+  Proof.
+    intros.
+    eapply af_iter with Ri (ltof _ (fun '(i, w) => f i w));
+      auto.
+    apply well_founded_ltof.
+  Qed.
+
+  Lemma af_iter_nat'{X I} Rr (f: I -> World E -> nat) (i: I) w (k: I -> ctree E (I + X)):
+    (forall (i: I) w,
+        not_done w ->
+        <( {k i}, w |= AF AX done
+                    {fun (x: I + X) w' =>
+                       match x with
+                       | inl i' => not_done w' /\ f i' w' < f i w
+                       | inr r' => Rr r' w'
+                       end})>) ->
+    not_done w ->
+    <( {iter k i}, w |= AF done Rr )>.
+  Proof.
+    intros.
+    eapply af_iter_nat with
+      (Ri:=fun _ => not_done) (f:=f); intros; auto.
+  Qed.
+
+  (* Well-founded induction on length of lists *)
+  Lemma af_iter_list{A X I} Ri Rr (f: I -> World E -> list A) (i: I) w (k: I -> ctree E (I + X)):
+    (forall (i: I) w,
+        Ri i w ->
+        <( {k i}, w |= AF AX done
+                    {fun (x: I + X) w' =>
+                       match x with
+                       | inl i' => Ri i' w' /\ length (f i' w') < length (f i w)
+                       | inr r' => Rr r' w'
+                       end})>) ->
+    Ri i w ->
+    <( {iter k i}, w |= AF done Rr )>.
+  Proof.
+    intros.
+    eapply af_iter_nat with
+      Ri (fun i w => length (f i w)); auto.
+  Qed.
+
+  Lemma af_iter_list'{A X I} Rr (f: I -> World E -> list A) (i: I) w (k: I -> ctree E (I + X)):
+    (forall (i: I) w,
+        not_done w ->
+        <( {k i}, w |= AF AX done
+                    {fun (x: I + X) w' =>
+                       match x with
+                       | inl i' => not_done w' /\
+                                    length (f i' w') < length (f i w)
+                       | inr r' => Rr r' w'
+                       end})>) ->
+    not_done w ->
+    <( {iter k i}, w |= AF done Rr )>.
+  Proof.
+    intros.
+    eapply af_iter_list with
+      (Ri:=fun _ => not_done) (f:=f); intros; auto.
+  Qed.  
+End CtlAfIter.
+
+(*| Combinators for [interp_state] |*)
+Section CtlAfState.
+  Context {E F S: Type} {HE: Encode E} {HF: Encode F}
+    (h: E ~> stateT S (ctree F)).
+
+  Theorem af_bind_state_vis{X Y}: forall s w (t: ctree E Y) (k: Y -> ctree E X) φ,
+      <( {interp_state h t s}, w |= AF vis φ )> ->
+      <( {interp_state h (x <- t ;; k x) s}, w |= AF vis φ )>.
+  Proof.
+    intros.
+    rewrite interp_state_bind.
+    now apply af_bind_vis.
+  Qed.
+  
+  Theorem af_bind_state_pure{X Y}: forall s w (t: ctree E Y) (k: Y -> ctree E X),
+      <( {interp_state h t s}, w |= AF pure )> ->
+      <( {interp_state h (x <- t ;; k x) s}, w |= AF pure )>.
+  Proof.
+    intros.
+    rewrite interp_state_bind.
+    now apply af_bind_pure.
+  Qed.
+
+  Theorem af_bind_state_r{X Y}: forall s (t: ctree E Y) (k: Y -> ctree E X) w φ (R: Y * S -> World F -> Prop),
+      <( {interp_state h t s}, w |= AF AX done R )> ->
+      (forall (y: Y) (s: S) w, R (y,s) w ->
+                    not_done w ->
+                    <( {interp_state h (k y) s}, w |= AF now φ )>) ->
+      <( {interp_state h (x <- t ;; k x) s}, w |= AF now φ )>.
+  Proof.
+    intros.
+    rewrite interp_state_bind.
+    apply af_bind_r with (R:=R); auto.
+    intros [y s'] w' Hr Hd; auto.
+  Qed.
+     
+  Theorem af_iter_state{X I} s Ri (Rr: rel (X * S) (World F))  Rv (i: I) (k: I -> ctree E (I + X)) w:
+    (forall (i: I) w s,
+        Ri i w s ->
+        <( {interp_state h (k i) s}, w |= AF AX done
+          {fun '(x, s') w' =>
+             match x with
+             | inl i' => Ri i' w' s'
+                        /\ Rv (i', w', s') (i, w, s)
+             | inr r' => Rr (r',s') w'
+             end})>) ->
+    well_founded Rv ->
+    Ri i w s ->
+    <( {interp_state h (Ctree.iter k i) s}, w |= AF done Rr )>.
+  Proof.
+    intros H WfR Hi.
+    generalize dependent k.
+    revert Hi.
+    remember (i, w, s) as P.
+    replace i with (fst (fst P)) by now subst.
+    replace w with (snd (fst P)) by now subst.
+    replace s with (snd P) by now subst.
+    clear HeqP i w s.
+    Opaque entailsF.
+    induction P using (well_founded_induction WfR);
+      destruct P as ((i, w), s); cbn in *. 
+    rename H into HindWf.
+    intros.
+    rewrite interp_state_unfold_iter.
+    eapply af_bind_r with (R:=fun '(r, s0) (w0 : World F) =>
+                      match r with
+                      | inl i' => Ri i' w0 s0 /\ Rv (i', w0, s0) (i, w, s)
+                      | inr r' => Rr (r',s0) w0
+                      end); auto.
+    intros ([i' | r] & s') w'; cbn.
+    - intros (Hi' & Hv) Hd.
+      apply af_guard.
+      remember (i', w',s') as y.
+      replace i' with (fst (fst y)) by now subst.
+      replace w' with (snd (fst y)) by now subst.
+      replace s' with (snd y) by now subst.      
+      apply HindWf; inv Heqy; auto.
+    - intros; apply af_ret; auto.
+  Qed.
+    
+  (*| Instead of a WF relation [Rv] provide a "ranking" function [f] |*)
+  Lemma af_iter_state_nat{X I} (s: S) Ri (Rr: rel (X * S) (World F)) (f: I -> World F -> S -> nat) (i: I) w
+    (k: I -> ctree E (I + X)):
+    (forall (i: I) w s,
+        Ri i w s ->
+        <( {interp_state h (k i) s}, w |= AF AX done
+                    {fun '(x, s') w' =>
+                       match x with
+                       | inl i' => Ri i' w' s' /\ f i' w' s' < f i w s
+                       | inr r' => Rr (r',s') w'
+                       end})>) ->
+    Ri i w s ->
+    <( {interp_state h (Ctree.iter k i) s}, w |= AF done Rr )>.
+  Proof.
+    intros.
+    eapply af_iter_state with Ri (ltof _ (fun '(i, w, s) => f i w s)); auto.
+    apply well_founded_ltof.
+  Qed.
+
+  Lemma af_iter_state_nat'{X I} (Rr: rel (X * S) (World F)) (f: I -> S -> nat) (s: S)
+    (i: I) w (k: I -> ctree E (I + X)):
+    (forall (i: I) w s,
+        not_done w ->
+        <( {interp_state h (k i) s}, w |= AF AX done
+                    {fun '(x, s') w' =>
+                       match x with
+                       | inl i' => not_done w' /\ f i' s' < f i s
+                       | inr r' => Rr (r',s') w'
+                       end})>) ->
+    not_done w ->
+    <( {interp_state h (Ctree.iter k i) s}, w |= AF done Rr )>.
+  Proof.
+    intros.
+    eapply af_iter_state_nat with (Ri:=fun _ w _ => not_done w) (f:=fun i _ => f i); auto.
+  Qed.
+End CtlAfState.
+
+(*| Combinators for [interp_state] with [writerE] |*)
+Section CtlAfStateList.
+  Context {E F A: Type} {HE: Encode E} {HF: Encode F} (h: E ~> stateT (list A) (ctree F)).
+
+  Lemma af_iter_state_list{X I} Ri (Rr: rel (X * list A) (World F)) (l: list A) w (i: I) (k: I -> ctree E (I + X)):
+    (forall (i: I) w (l: list A),
+        Ri i w l ->
+        <( {interp_state h (k i) l}, w |= AF AX done
+                 {fun '(x, l') w' =>
+                    match x with
+                    | inl i' => Ri i' w' l' /\ length l' < length l
+                    | inr r' => Rr (r', l') w'
+                    end})>) ->
+    Ri i w l ->
+    <( {interp_state h (Ctree.iter k i) l}, w |= AF done Rr )>.
+  Proof.
+    intros.
+    apply af_iter_state_nat with (Ri:=Ri) (f:=fun _ _ l => length l); auto.
+  Qed.
+
+  Lemma af_iter_state_list'{X I} (Rr: rel (X * list A) (World F)) (l: list A) (i: I) w (k: I -> ctree E (I + X)):
+    (forall (i: I) w (l: list A),
+        not_done w ->
+        <( {interp_state h (k i) l}, w |= AF AX done
+             {fun '(x, l') w' =>
+                match (x: I + X) with
+                | inl _ => not_done w' /\ length l' < length l
+                | inr r' => Rr (r',l') w'
+                end})>) ->
+    not_done w ->
+    <( {interp_state h (Ctree.iter k i) l}, w |= AF done Rr )>.
+  Proof.
+    intros.
+    eapply af_iter_state_list with (Ri:=fun _ w _ => not_done w); auto.
+  Qed.
+
+End CtlAfStateList.  
